Compiles, without one admit in SemProps

theories/Parameters.v
@@ -1,4 +1,4 @@
-Require Import sflib.
+Require Import CoqlibC.
 Require Import List.
 Require Import LinkingC.
 
@@ -44,6 +44,7 @@ Module Values.
     Vundef: val;
     int: Type;
     Vint: int -> val;
+    Vint_inj: forall a b, Vint a = Vint b -> a = b;
   }
   .
 End Values.
@@ -68,7 +69,7 @@ End Mem.
 Definition mem `{Mem.class}: Type := Mem.t.
 
 Module Senv.
-  Class class `{AST.class}: Type := {
+  Class class `{AC: AST.class}: Type := {
     t: Type;
     public_symbol: t -> AST.ident -> bool;
   }
@@ -98,13 +99,25 @@ Module Sk.
     Linker:> Linker t;
     load_skenv: t -> Genv.t (fundef signature) unit;
     load_mem: t -> option mem;
+    link_preserves_wf_sk: forall
+        sk0 sk1 sk_link
+        (WFSK0: wf sk0)
+        (WFSK1: wf sk1)
+        (LINK: link sk0 sk1 = Some sk_link)
+      ,
+        (<<WF: wf sk_link>>)
+    ;
   }
   .
 End Sk.
 Definition prog_main `{Sk.class} := Sk.prog_main.
 
 Module SkEnv.
-  Class class `{Sk.class} `{Genv.class}: Type := {
+  (*** NOTE: put `{Genv.class} and you get an error, because there are multiple instances of Genv.class
+             (one required by Sk.class and the other)
+       TODO: Avoid such thing systematically?
+   ***)
+  Class class `{Sk.class}: Type := {
     t: Type := Genv.t (fundef signature) unit;
     wf: t -> Prop;
     wf_mem: t -> Sk.t -> mem -> Prop;
@@ -113,8 +126,27 @@ Module SkEnv.
     project_spec: t -> Sk.t -> t -> Prop;
     includes: t -> Sk.t -> Prop;
     project_impl_spec: forall skenv sk (INCL: includes skenv sk),
-        <<PROJ: project_spec skenv sk (project skenv sk)>>;
+        (<<PROJ: project_spec skenv sk (project skenv sk)>>);
+    linkorder_includes: forall
+        (sk0 sk1: Sk.t)
+        (LO: linkorder sk0 sk1)
+      ,
+        (<<INCL: includes (Sk.load_skenv sk1) sk0>>);
     empty: t;
+    load_skenv_wf: forall
+        sk
+        (WF: Sk.wf sk)
+      ,
+        (<<WF: wf (Sk.load_skenv sk)>>)
+    ;
+    load_skenv_wf_mem: forall
+        sk_link m_init
+        (WF: Sk.wf sk_link)
+        (LOADM: Sk.load_mem sk_link = Some m_init)
+      ,
+        let skenv_link := Sk.load_skenv sk_link in
+        <<WFM: forall sk (WF: Sk.wf sk) (LO: linkorder sk sk_link), wf_mem skenv_link sk m_init>>
+    ;
   }
   .
 End SkEnv.
@@ -122,12 +154,13 @@ End SkEnv.
 Coercion SkEnv.to_senv: SkEnv.t >-> Senv.t.
 
 Module Events.
-  Class class `{Values.class} `{Mem.class} `{Senv.class}: Type := {
+  Class class `{VC: Values.class} `{MC: Mem.class} `{SC: Senv.class}: Type := {
     event: Type;
     trace := list event;
     Eapp: trace -> trace -> trace := @app _;
     E0: trace := nil;
     match_traces: Senv.t -> trace -> trace -> Prop;
+    match_traces_nil_nil: forall se, match_traces se E0 E0;
     match_traces_nil_l: forall
         se t
         (MATCH: match_traces se E0 t)
@@ -160,14 +193,150 @@ Module Events.
         match_traces ge t1 t2;
   }
   .
+  Section Events.
+    Context `{EC: Events.class}.
+
+    CoInductive traceinf : Type :=
+    | Econsinf: event -> traceinf -> traceinf.
+
+    Fixpoint Eappinf (t: trace) (T: traceinf) {struct t} : traceinf :=
+      match t with
+      | nil => T
+      | ev :: t' => Econsinf ev (Eappinf t' T)
+      end.
+
+    Infix "**" := Eapp (at level 60, right associativity).
+    Infix "***" := Eappinf (at level 60, right associativity).
+
+    Lemma E0_left: forall t, E0 ** t = t.
+    Proof. auto. Qed.
+
+    Lemma E0_right: forall t, t ** E0 = t.
+    Proof. intros. unfold E0, Eapp. rewrite <- app_nil_end. auto. Qed.
+
+    Lemma Eapp_assoc: forall t1 t2 t3, (t1 ** t2) ** t3 = t1 ** (t2 ** t3).
+    Proof. intros. unfold Eapp, trace. apply app_ass. Qed.
+
+    Lemma Eapp_E0_inv: forall t1 t2, t1 ** t2 = E0 -> t1 = E0 /\ t2 = E0.
+    Proof (@app_eq_nil event).
+
+    Lemma E0_left_inf: forall T, E0 *** T = T.
+    Proof. auto. Qed.
+
+    Lemma Eappinf_assoc: forall t1 t2 T, (t1 ** t2) *** T = t1 *** (t2 *** T).
+    Proof.
+      induction t1; intros; simpl. auto. f_equal; auto.
+    Qed.
+
+    Hint Rewrite E0_left E0_right Eapp_assoc
+         E0_left_inf Eappinf_assoc: trace_rewrite.
+
+    Opaque trace E0 Eapp Eappinf.
+
+    Ltac substTraceHyp :=
+      match goal with
+      | [ H: (@eq trace ?x ?y) |- _ ] =>
+        subst x || clear H
+      end.
+
+    Ltac decomposeTraceEq :=
+      match goal with
+      | [ |- (_ ** _) = (_ ** _) ] =>
+        apply (f_equal2 Eapp); auto; decomposeTraceEq
+      | _ =>
+        auto
+      end.
+
+    Ltac traceEq :=
+      repeat substTraceHyp; autorewrite with trace_rewrite; decomposeTraceEq.
+
+    CoInductive traceinf': Type :=
+    | Econsinf': forall (t: trace) (T: traceinf'), t <> E0 -> traceinf'.
+    Arguments Econsinf': clear implicits.
+
+    Program Definition split_traceinf' (t: trace) (T: traceinf') (NE: t <> E0): event * traceinf' :=
+      match t with
+      | nil => _
+      | e :: nil => (e, T)
+      | e :: t' => (e, Econsinf' t' T _)
+      end.
+    Next Obligation.
+      elimtype False. elim NE. auto.
+    Qed.
+    Next Obligation.
+      red; intro. elim (H e). rewrite H0. auto.
+    Qed.
+    Arguments split_traceinf': clear implicits.
+
+    CoFixpoint traceinf_of_traceinf' (T': traceinf') : traceinf :=
+      match T' with
+      | Econsinf' t T'' NOTEMPTY =>
+        let (e, tl) := split_traceinf' t T'' NOTEMPTY in
+        Econsinf e (traceinf_of_traceinf' tl)
+      end.
+
+    Remark unroll_traceinf':
+      forall T, T = match T with Econsinf' t T' NE => Econsinf' t T' NE end.
+    Proof.
+      intros. destruct T; auto.
+    Qed.
+
+    Remark unroll_traceinf:
+      forall T, T = match T with Econsinf t T' => Econsinf t T' end.
+    Proof.
+      intros. destruct T; auto.
+    Qed.
+
+    Lemma traceinf_traceinf'_app:
+      forall t T NE,
+        traceinf_of_traceinf' (Econsinf' t T NE) = t *** traceinf_of_traceinf' T.
+    Proof.
+      induction t.
+      intros. elim NE. auto.
+      intros. simpl.
+      rewrite (unroll_traceinf (traceinf_of_traceinf' (Econsinf' (a :: t) T NE))).
+      simpl. destruct t. auto.
+      Transparent Eappinf.
+      simpl. f_equal. apply IHt.
+    Qed.
+
+    (** Prefixes of traces. *)
+
+    Definition trace_prefix (t1 t2: trace) :=
+      exists t3, t2 = t1 ** t3.
+
+    Definition traceinf_prefix (t1: trace) (T2: traceinf) :=
+      exists T3, T2 = t1 *** T3.
+
+    Lemma trace_prefix_app:
+      forall t1 t2 t,
+        trace_prefix t1 t2 ->
+        trace_prefix (t ** t1) (t ** t2).
+    Proof.
+      intros. destruct H as [t3 EQ]. exists t3. traceEq.
+    Qed.
+
+    Lemma traceinf_prefix_app:
+      forall t1 T2 t,
+        traceinf_prefix t1 T2 ->
+        traceinf_prefix (t ** t1) (t *** T2).
+    Proof.
+      intros. destruct H as [T3 EQ]. exists T3. subst T2. traceEq.
+    Qed.
+
+
+  End Events.
 End Events.
 
 Export Events.
 
 
 
-
-
+(****************************************************************************************)
+(****************************************************************************************)
+(****************************************************************************************)
+(****************************************************************************************)
+(****************************************************************************************)
 
 Class PARAMETERS: Type := {
   Mem_class:> Mem.class;
@@ -184,50 +353,40 @@ Class PARAMETERS: Type := {
 
 Context {PRMS: PARAMETERS}.
 
-Check Mem.empty.
-Check Senv.t.
+(****************************************************************************************)
+(****************************************************************************************)
+(****************************************************************************************)
+(****************************************************************************************)
+(****************************************************************************************)
 
 
+
+(** TODO: Can we remove this redundancy **)
+Arguments Econsinf' {_} {_} {_} {_} {_}.
+Arguments split_traceinf' {_} {_} {_} {_} {_}.
 
 Infix "**" := Eapp (at level 60, right associativity).
-
-Lemma E0_left: forall t, E0 ** t = t.
-Proof. auto. Qed.
-
-Lemma E0_right: forall t, t ** E0 = t.
-Proof. intros. unfold E0, Eapp. rewrite <- app_nil_end. auto. Qed.
-
-Lemma Eapp_assoc: forall t1 t2 t3, (t1 ** t2) ** t3 = t1 ** (t2 ** t3).
-Proof. intros. unfold Eapp, trace. apply app_ass. Qed.
-
-Lemma Eapp_E0_inv: forall t1 t2, t1 ** t2 = E0 -> t1 = E0 /\ t2 = E0.
-Proof (@app_eq_nil event).
-
-(* Lemma E0_left_inf: forall T, E0 *** T = T. *)
-(* Proof. auto. Qed. *)
-
-(* Lemma Eappinf_assoc: forall t1 t2 T, (t1 ** t2) *** T = t1 *** (t2 *** T). *)
-(* Proof. *)
-(*   induction t1; intros; simpl. auto. decEq; auto. *)
-(* Qed. *)
+Infix "***" := Eappinf (at level 60, right associativity).
 
 Hint Rewrite E0_left E0_right Eapp_assoc
-             (* E0_left_inf Eappinf_assoc *)
-  : trace_rewrite.
+     E0_left_inf Eappinf_assoc: trace_rewrite.
 
 Ltac substTraceHyp :=
   match goal with
   | [ H: (@eq trace ?x ?y) |- _ ] =>
-       subst x || clear H
+    subst x || clear H
   end.
 
 Ltac decomposeTraceEq :=
   match goal with
   | [ |- (_ ** _) = (_ ** _) ] =>
-      apply (f_equal2 app); auto; decomposeTraceEq
+    apply (f_equal2 Eapp); auto; decomposeTraceEq
   | _ =>
-      auto
+    auto
   end.
 
 Ltac traceEq :=
   repeat substTraceHyp; autorewrite with trace_rewrite; decomposeTraceEq.
+(** TODOEND **)
+
+
