theories/AdequacySound.v
@@ -1,0 +1,266 @@
+Require Import Parameters.
+Require Import CoqlibC.
+Require Import Simulation.
+Require Import LinkingC.
+Require Import Smallstep.
+
+Require Import ModSem Mod Sem.
+Require Import SimSymb SimMem SimMod SimModSem SimProg (* SimLoad *) SimProg.
+Require Import SemProps Ord.
+Require Import Sound Preservation.
+
+Set Implicit Arguments.
+
+
+
+
+Section ADQSOUND.
+
+  Context `{SM: SimMem.class}.
+  Context {SS: SimSymb.class SM}.
+  Context `{SU: Sound.class}.
+
+  Variable pp: ProgPair.t.
+  Hypothesis SIMPROG: ProgPair.sim pp.
+  Let p_src := (ProgPair.src pp).
+  Let p_tgt := (ProgPair.tgt pp).
+  Hypothesis (WFSKSRC: forall md (IN: In md p_src), <<WF: Sk.wf md>>).
+  Hypothesis (WFSKTGT: forall md (IN: In md p_tgt), <<WF: Sk.wf md>>).
+
+  Variable sk_link_src sk_link_tgt: Sk.t.
+  Hypothesis LINKSRC: (link_sk p_src) = Some sk_link_src.
+  Hypothesis LINKTGT: (link_sk p_tgt) = Some sk_link_tgt.
+  Let sem_src := Sem.sem p_src.
+  Let sem_tgt := Sem.sem p_tgt.
+
+  Let skenv_link_src := (Sk.load_skenv sk_link_src).
+  Let skenv_link_tgt := (Sk.load_skenv sk_link_tgt).
+
+  Variable ss_link: SimSymb.t.
+  Hypothesis (SIMSKENV: exists sm, SimSymb.sim_skenv sm ss_link skenv_link_src skenv_link_tgt).
+
+  Hypothesis INCLSRC: forall mp (IN: In mp pp), SkEnv.includes skenv_link_src (Mod.sk mp.(ModPair.src)).
+  Hypothesis INCLTGT: forall mp (IN: In mp pp), SkEnv.includes skenv_link_tgt (Mod.sk mp.(ModPair.tgt)).
+  Hypothesis SSLE: forall mp (IN: In mp pp), SimSymb.le mp.(ModPair.ss) ss_link.
+
+  Let WFSKLINKSRC: Sk.wf sk_link_src. eapply link_list_preserves_wf_sk; et. Qed.
+  Let WFSKLINKTGT: Sk.wf sk_link_tgt. eapply link_list_preserves_wf_sk; et. Qed.
+
+  (* Let ge: Ge.t := sem_src.(Smallstep.globalenv). *)
+
+  Inductive sound_ge (su0: Sound.t) (m0: mem): Prop :=
+  | sound_ge_intro
+      (GE: Forall (fun ms => su0.(Sound.skenv) m0 ms.(ModSem.skenv) /\ su0.(Sound.skenv) m0 ms.(ModSem.skenv_link))
+                  (fst sem_src.(Smallstep.globalenv)))
+  .
+
+  Lemma lepriv_preserves_sound_ge
+        m0 su0 su1
+        (GE: sound_ge su0 m0)
+        (LE: Sound.lepriv su0 su1):
+      <<GE: sound_ge su1 m0>>.
+  Proof.
+    inv GE. econs; eauto. rewrite Forall_forall in *. ii. split; eapply Sound.skenv_lepriv; try apply GE0; eauto.
+  Qed.
+
+  Lemma hle_preserves_sound_ge
+        m0 su0 su1
+        (WF: Sound.wf su0)
+        (GE: sound_ge su0 m0)
+        (LE: Sound.hle su0 su1):
+      <<GE: sound_ge su1 m0>>.
+  Proof.
+    eapply lepriv_preserves_sound_ge; eauto. eapply Sound.hle_lepriv; et.
+  Qed.
+
+  Lemma mle_preserves_sound_ge
+        m0 m1 su0
+        (GE: sound_ge su0 m0)
+        (LE: Sound.mle su0 m0 m1):
+      <<GE: sound_ge su0 m1>>.
+  Proof.
+    inv GE. econs; eauto. rewrite Forall_forall in *. ii. split; eapply Sound.skenv_mle; try apply GE0; eauto.
+  Qed.
+
+  (* stack can go preservation when su0 is given *)
+  Inductive sound_stack (args: Args.t): list Frame.t -> Prop :=
+  | sound_stack_nil
+      (EXSU: exists su_ex, Sound.args su_ex args /\ sound_ge su_ex (Args.get_m args)):
+      sound_stack args []
+  | sound_stack_cons
+      args_tail tail ms lst0
+      (TL: sound_stack args_tail tail)
+      (FORALLSU: forall su0
+          (SUARGS: Sound.args su0 args_tail)
+          (SUGE: sound_ge su0 (Args.get_m args_tail)),
+          (<<HD: forall
+                 sound_state_all
+                 (PRSV: local_preservation_noguarantee ms sound_state_all),
+                 <<SUST: sound_state_all su0 (Args.get_m args_tail) lst0>>>>)
+          /\
+          (<<K: forall
+                 sound_state_all
+                 (PRSV: local_preservation_noguarantee ms sound_state_all),
+                 (* (<<SUST: sound_state_all su0 args.(Args.get_m) lst0>>) *)
+                 (* /\ *)
+                 exists su_gr,
+                   (<<ARGS: Sound.args su_gr args>>) /\
+                   (<<LE: Sound.lepriv su0 su_gr>>) /\
+                   (<<K: forall retv lst1 su_ret
+                       (LE: Sound.hle su_gr su_ret)
+                       (SURETV: Sound.retv su_ret retv)
+                       (MLE: Sound.mle su_gr (Args.get_m args) (Retv.get_m retv))
+                       (AFTER: ms.(ModSem.after_external) lst0 retv lst1),
+                       (* sound_state_all su0 args.(Args.get_m) lst1>>) *)
+                       sound_state_all su0 (Args.get_m args_tail) lst1>>)
+             >>)
+          /\
+          (<<MLE: Sound.mle su0 (Args.get_m args_tail) (Args.get_m args)>>)
+      )
+      (EXSU: exists su_ex, Sound.args su_ex args_tail /\ sound_ge su_ex (Args.get_m args_tail))
+      (EX: exists sound_state_ex, local_preservation ms sound_state_ex):
+      sound_stack args ((Frame.mk ms lst0) :: tail).
+
+  Inductive sound_state: state -> Prop :=
+  | sound_state_normal
+      args_tail tail ms lst0 m_arg
+      (TL: sound_stack args_tail tail)
+      (EXSU: exists su_ex, Sound.args su_ex args_tail /\ sound_ge su_ex m_arg)
+      (FORALLSU: forall su0
+          (SUARGS: Sound.args su0 args_tail)
+          (SUGE: sound_ge su0 (Args.get_m args_tail)),
+          (<<HD: forall
+              sound_state_all
+              (PRSV: local_preservation_noguarantee ms sound_state_all),
+              <<SUST: sound_state_all su0 m_arg lst0>>>>))
+      (EX: exists sound_state_ex, local_preservation ms sound_state_ex)
+      (ABCD: (Args.get_m args_tail) = m_arg)
+    :
+      sound_state (State ((Frame.mk ms lst0) :: tail))
+  | sound_state_call
+      m_tail frs args
+      (* (ARGS: Sound.args su0 args) *)
+      (STK: sound_stack args frs)
+      (* (MLE: Sound.mle su0 m_tail args.(Args.get_m)) *)
+      (EQ: (Args.get_m args) = m_tail)
+      (EXSU: exists su_ex, Sound.args su_ex args /\ sound_ge su_ex m_tail):
+      sound_state (Callstate args frs).
+
+  Lemma sound_init
+        st0
+        (INIT: sem_src.(Smallstep.initial_state) st0):
+    <<SU: sound_state st0>>.
+  Proof.
+    inv INIT. clarify. clear skenv_link_tgt p_tgt skenv_link_tgt sem_tgt LINKTGT INCLTGT WFSKTGT SIMSKENV.
+    hexploit Sound.init_spec; eauto. i; des. esplits; eauto.
+    assert(WFSKE: SkEnv.wf (Sk.load_skenv sk_link_src)).
+    { eapply SkEnv.load_skenv_wf; et. }
+    assert(GE: sound_ge su_init m_init).
+    { econs. rewrite Forall_forall. intros ? IN. ss. des_ifs. u in IN.
+      rewrite in_map_iff in IN. des; ss; clarify.
+      + s. split; try eapply Sound.system_skenv; eauto.
+      + assert(INCL: SkEnv.includes (Sk.load_skenv sk_link_src) (Mod.sk x0)).
+        { unfold p_src in IN0. unfold ProgPair.src in *. rewrite in_map_iff in IN0. des. clarify. eapply INCLSRC; et. }
+        split; ss.
+        * eapply Sound.skenv_project; eauto.
+          { eapply link_load_skenv_wf_mem; et. }
+          rewrite <- Mod.get_modsem_skenv_spec; ss. eapply SkEnv.project_impl_spec; et.
+        * rewrite Mod.get_modsem_skenv_link_spec. ss.
+    }
+    econs; eauto. econs; eauto.
+    (* - eapply Sound.greatest_adq; eauto. *)
+    (* - econs; eauto. *)
+    (* - eapply vle_preserves_sound_ge; eauto. *)
+    (*   eapply Sound.greatest_adq; eauto. *)
+  Unshelve.
+    all: ss.
+  Qed.
+
+  Lemma sound_progress
+        st0 tr st1
+        (SUST: sound_state st0)
+        (STEP: Step sem_src st0 tr st1):
+      <<SUST: sound_state st1>>.
+  Proof.
+    inv STEP.
+    - (* CALL *)
+      inv SUST. ss. des. exploit FORALLSU; eauto. { eapply local_preservation_noguarantee_weak; eauto. } intro T; des.
+      inv EX. exploit CALL; eauto. i; des. esplits; eauto. econs; eauto; cycle 1.
+      + esplits; eauto. eapply lepriv_preserves_sound_ge; eauto.
+        { eapply mle_preserves_sound_ge; eauto. }
+      + econs; eauto; cycle 1.
+        { esplits; eauto. econs; eauto. }
+        ii. esplits; eauto.
+        * ii. exploit FORALLSU; try apply SUARGS; eauto.
+        * ii. exploit FORALLSU; try apply SUARGS; eauto. intro U; des.
+          inv PRSV. exploit CALL0; eauto. i; des. esplits; eauto. ii. eapply K0; eauto.
+        * exploit FORALLSU; eauto.
+          { eapply local_preservation_noguarantee_weak; eauto. econs; eauto. }
+          i; des. exploit CALL; eauto. i; des. ss.
+    - (* INIT *)
+      inv SUST. ss. des_ifs. esplits; eauto. econs; eauto.
+      + ii. esplits; eauto.
+        * ii. inv PRSV. inv SUGE. rewrite Forall_forall in *.
+          exploit GE; eauto. { ss. des_ifs. eapply MSFIND. } intro T; des. eapply INIT0; et.
+      + inv MSFIND. ss. rr in SIMPROG. rewrite Forall_forall in *. des; clarify.
+        { eapply system_local_preservation. }
+        u in MODSEM. rewrite in_map_iff in MODSEM. des; clarify. rename x into md_src.
+        assert(exists mp, In mp pp /\ mp.(ModPair.src) = md_src).
+        { clear - MODSEM0. rr in pp. rr in p_src. subst p_src. rewrite in_map_iff in *. des. eauto. }
+        des. exploit SIMPROG; eauto. intros MPSIM. inv MPSIM.
+        destruct SIMSKENV. exploit SIMMS.
+        { eapply INCLSRC; et. }
+        { eapply INCLTGT; et. }
+        { eapply SkEnv.load_skenv_wf; et. }
+        { eapply SkEnv.load_skenv_wf; et. }
+        { eapply SSLE; eauto. }
+        { eauto. }
+        intro SIM; des. inv SIM. ss. esplits; eauto.
+    - (* INTERNAL *)
+      inv SUST. ss. esplits; eauto. econs; eauto. i. des.
+      exploit FORALLSU; eauto. { eapply local_preservation_noguarantee_weak; eauto. } intro U; des. esplits; eauto. i. ss. inv PRSV.
+      eapply STEP; eauto.
+      + eapply FORALLSU; eauto. econs; eauto.
+      + split; ii; ModSem.tac.
+    - (* RETURN *)
+      inv SUST. ss. rename ms into ms_top. rename args_tail into args_tail_top.
+      inv TL. ss. unfold Frame.update_st. s. des. esplits; eauto. econs; eauto. ii. esplits; eauto.
+      + ii. exploit FORALLSU0; eauto. i; des. exploit K; eauto. i; des. inv EX.
+        exploit RET; eauto.
+        { eapply FORALLSU; eauto.
+          { eapply lepriv_preserves_sound_ge. { eapply mle_preserves_sound_ge; eauto. } eauto. }
+          { eapply local_preservation_noguarantee_weak; eauto. econs; et. } }
+        i; des.
+        eapply K0; eauto.
+  Unshelve.
+    all: ss.
+  Qed.
+
+  (* Lemma sound_progress_star *)
+  (*       st0 tr st1 *)
+  (*       (SUST: sound_state st0) *)
+  (*       (STEP: Star sem_src st0 tr st1): *)
+  (*     <<SUST: sound_state st1>>. *)
+  (* Proof. *)
+  (*   induction STEP. *)
+  (*   - esplits; eauto. *)
+  (*   - clarify. i. exploit sound_progress; eauto. *)
+  (* Qed. *)
+
+  (* Lemma sound_progress_plus *)
+  (*       st0 tr st1 *)
+  (*       (SUST: sound_state st0) *)
+  (*       (STEP: Plus sem_src st0 tr st1): *)
+  (*     <<SUST: sound_state st1>>. *)
+  (* Proof. *)
+  (*   eapply sound_progress_star; eauto. eapply plus_star; eauto. *)
+  (* Qed. *)
+
+  Theorem preservation: @preservation sem_src sound_state.
+  Proof.
+    econs.
+    - eapply sound_init.
+    - eapply sound_progress.
+  Qed.
+
+End ADQSOUND.
