theories/SemProps.v
@@ -1,0 +1,359 @@
+Require Import Parameters.
+Require Import CoqlibC.
+Require Import LinkingC.
+Require Import JMeq.
+Require Import Smallstep.
+Require Import Simulation.
+
+Require Import BehaviorsC.
+Require Import ModSem Mod Sem.
+Require Import SimSymb SimMem.
+
+Require Import ModSemProps.
+
+Set Implicit Arguments.
+
+
+(* TODO: better namespace? *)
+Lemma includes_refl
+      sk:
+    <<INCL: SkEnv.includes (Sk.load_skenv sk) sk>>.
+Proof.
+  eapply SkEnv.linkorder_includes; et.
+  eapply linkorder_refl.
+Qed.
+
+
+
+
+Lemma link_includes
+      p sk_link_src
+      (LINK: link_sk p = Some sk_link_src)
+      md
+      (IN: In md p):
+    SkEnv.includes (Sk.load_skenv sk_link_src) (Mod.sk md).
+Proof.
+  unfold link_sk in *.
+  (* TODO: can we remove `_ LINK` ? *)
+  (* Arguments link_list_linkorder [_]. *)
+  (* Arguments link_list_linkorder: default implicits. *)
+  hexploit (link_list_linkorder _ LINK); et. intro LOS; des.
+  rewrite Forall_forall in *. exploit (LOS md); et.
+  { rewrite in_map_iff. esplits; et. }
+  intro LO.
+  eapply SkEnv.linkorder_includes; et.
+Qed.
+
+Theorem link_list_preserves_wf_sk
+        p sk_link
+        (LINK: link_sk p = Some sk_link)
+        (WFSK: forall md, In md p -> <<WF: Sk.wf md >>):
+    <<WF: Sk.wf sk_link>>.
+Proof.
+  unfold link_sk in *. ginduction p; ii; ss. unfold link_list in LINK. des_ifs_safe. ss.
+  destruct (link_list_aux (map Mod.sk p)) eqn:T; ss.
+  { clarify. destruct p; ss; des_ifs. eapply WFSK. eauto. }
+  des_ifs. rename t into tl. rename a into hd. specialize (IHp tl). exploit IHp; eauto.
+  { unfold link_list. des_ifs. }
+  i; des. eapply (Sk.link_preserves_wf_sk hd tl); et. eapply WFSK; et.
+Qed.
+
+
+
+Section INITDTM.
+
+ (* Lemma link_sk_disjoint *)
+ (*        md0 md1 p0 id skenv_link b if_sig if_sig0 restl sk_link gd_big0 *)
+ (*        (IN : In md0 p0) *)
+ (*        (NOTSAME : md0 <> md1) *)
+ (*        (DEFS1 : defs (Mod.get_sk md1 (Mod.data md1)) id) *)
+ (*        (DEFS0 : defs (Mod.get_sk md0 (Mod.data md0)) id) *)
+ (*        (DEFBIG0 : Genv.find_def skenv_link b = Some gd_big0) *)
+ (*        (SYMBBIG0 : Genv.find_symbol skenv_link id = Some b) *)
+ (*        (WFBIG : SkEnv.wf skenv_link) *)
+ (*        (DEF0 : Genv.find_def (ModSem.skenv (Mod.get_modsem md0 skenv_link (Mod.data md0))) b = Some (Gfun (Internal if_sig))) *)
+ (*        (DEF1 : Genv.find_def (ModSem.skenv (Mod.get_modsem md1 skenv_link (Mod.data md1))) b = Some (Gfun (Internal if_sig0))) *)
+ (*        (INCLS : forall md : Mod.t, md1 = md \/ In md p0 -> SkEnv.includes skenv_link (Mod.get_sk md (Mod.data md))) *)
+ (*        (TL : link_list (map (fun md : Mod.t => Mod.get_sk md (Mod.data md)) p0) = Some restl) *)
+ (*        (HD : link (Mod.get_sk md1 (Mod.data md1)) restl = Some sk_link) *)
+ (*        (SKLINK : link_list (Mod.get_sk md1 (Mod.data md1) :: map (fun md : Mod.t => Mod.get_sk md (Mod.data md)) p0) = Some sk_link) *)
+ (*        (TLORD : Forall (fun x : Sk.t => linkorder x restl) (map (fun md : Mod.t => Mod.get_sk md (Mod.data md)) p0)) *)
+ (*        (HDORD : linkorder (Mod.get_sk md1 (Mod.data md1)) sk_link) *)
+ (*        (HDORD0 : linkorder restl sk_link): *)
+ (*      False. *)
+ (*  Proof. *)
+ (*    rewrite <- Mod.get_modsem_skenv_spec in *. rewrite Forall_forall in TLORD. *)
+ (*    assert (In (Mod.get_sk md0 (Mod.data md0)) (map (fun md : Mod.t => Mod.get_sk md (Mod.data md)) p0)). *)
+ (*    { rewrite in_map_iff. exists md0. auto. } *)
+ (*    assert (linkorder (Mod.get_sk md0 (Mod.data md0)) restl). *)
+ (*    { exploit TLORD; eauto. } *)
+ (*    Local Transparent Linker_prog. *)
+
+ (*    exploit INCLS; eauto. intros INCL0. inversion WFBIG. *)
+ (*    exploit DEFSYMB; eauto. i. des. *)
+ (*    exploit SkEnv.project_impl_spec; eauto. i. inv H2. *)
+ (*    exploit SYMBKEEP; eauto. i. *)
+
+ (*    assert (INTERN0: exists int_sig, Maps.PTree.get id (prog_defmap (Mod.get_sk md0 (Mod.data md0))) = Some (Gfun (Internal int_sig))). *)
+ (*    { rewrite SYMBBIG0 in H2. exploit DEFKEPT. eapply Genv.find_invert_symbol. eapply SYMBBIG0. eauto. i. des. eauto. } des. *)
+
+ (*    exploit (@prog_defmap_linkorder (fundef signature) unit). eapply H0. *)
+ (*    instantiate (2:=id). *)
+ (*    eauto. i. des. *)
+
+ (*    exploit INCLS. instantiate (1:=md1). auto. intros INCL1. *)
+ (*    exploit SkEnv.project_impl_spec; eauto. i. inv H5. *)
+ (*    exploit SYMBKEEP; eauto. i. *)
+
+ (*    assert (INTERN1: exists int_sig, Maps.PTree.get id (prog_defmap (Mod.get_sk md1 (Mod.data md1))) = Some (Gfun (Internal int_sig))). *)
+ (*    { rewrite SYMBBIG0 in H5. exploit DEFKEPT0. eapply Genv.find_invert_symbol. eapply SYMBBIG0. eauto. i. des. eauto. } des. *)
+
+ (*    exploit (@prog_defmap_linkorder (fundef signature) unit). eapply HDORD. *)
+ (*    instantiate (2:=id). *)
+ (*    eauto. i. des. *)
+
+ (*    Local Transparent Linker_def. simpl in *. inv H4. inv H9. Local Transparent Linker_fundef. *)
+ (*    simpl in *. inv H7. inv H8. inv HD. unfold link_prog in H7. des_ifs. *)
+ (*    symmetry in Heq. eapply andb_true_eq in Heq. des. *)
+ (*    symmetry in Heq0. rewrite Maps.PTree_Properties.for_all_correct in Heq0. unfold defs in *. exploit Heq0. eauto. i. *)
+ (*    unfold link_prog_check in H8. des_ifs. ss. rewrite andb_false_r in H8. clarify. *)
+ (*  Qed. *)
+
+  Context `{SM: SimMem.class}.
+  Context {SS: SimSymb.class SM}.
+  Variable p: program.
+  Hypothesis (WFSK: forall md (IN: In md p), <<WF: Sk.wf md>>).
+  Let sem := Sem.sem p.
+
+  Lemma find_fptr_owner_determ
+        fptr ms0 ms1
+        (FIND0: Ge.find_fptr_owner sem.(globalenv) fptr ms0)
+        (FIND1: Ge.find_fptr_owner sem.(globalenv) fptr ms1):
+      ms0 = ms1.
+  Proof.
+    admit "".
+  Qed.
+
+  Theorem initial_state_determ
+          st_init0 st_init1
+          (INIT0: sem.(Smallstep.initial_state) st_init0)
+          (INIT1: sem.(Smallstep.initial_state) st_init1):
+      st_init0 = st_init1.
+  Proof.
+    ss. inv INIT0; inv INIT1; ss. clarify.
+  Qed.
+
+End INITDTM.
+
+
+
+
+Lemma lift_step
+      (ms: ModSem.t) st0 tr st1
+      (STEP: Step ms st0 tr st1):
+    forall prog tail,
+    <<STEP: Step (Sem.sem prog)
+                 (State ((Frame.mk ms st0) :: tail)) tr
+                 (State ((Frame.mk ms st1) :: tail))>>.
+Proof. ii. econs 3; eauto. Qed.
+
+Lemma lift_star
+      (ms: ModSem.t) st0 tr st1
+      (STAR: Star ms st0 tr st1):
+    forall prog tail,
+    <<STAR: Star (Sem.sem prog) (State ((Frame.mk ms st0) :: tail)) tr (State ((Frame.mk ms st1) :: tail))>>.
+Proof.
+  ii. ginduction STAR; ii; ss.
+  - econs 1; eauto.
+  - clarify. econs 2; eauto.
+    + eapply lift_step; eauto.
+    + eapply IHSTAR; eauto.
+Qed.
+
+Lemma lift_plus
+      (ms: ModSem.t) st0 tr st1
+      (PLUS: Plus ms st0 tr st1):
+    forall prog tail,
+    <<PLUS: Plus (Sem.sem prog) (State ((Frame.mk ms st0) :: tail)) tr (State ((Frame.mk ms st1) :: tail))>>.
+Proof.
+  i. inv PLUS; ii; ss. econs; eauto.
+  - eapply lift_step; eauto.
+  - eapply lift_star; eauto.
+Qed.
+
+Lemma lift_dstep
+      (ms: ModSem.t) st0 tr st1 prog
+      (PUBEQ: ms.(symbolenv).(Senv.public_symbol) = (Sem.sem prog).(symbolenv).(Senv.public_symbol))
+      (DSTEP: DStep ms st0 tr st1):
+    forall tail,
+    <<DSTEP: DStep (Sem.sem prog) (State ((Frame.mk ms st0) :: tail)) tr (State ((Frame.mk ms st1) :: tail))>>.
+Proof.
+  ii. destruct DSTEP as [DTM STEP]. econs; eauto; cycle 1.
+  - econs; ss; eauto.
+  - inv DTM. econs; eauto.
+    + ii. ss. inv H; ss; ModSem.tac. inv H0; ss; ModSem.tac. clear STEP.
+      determ_tac sd_determ_at. esplits; auto.
+      * eapply match_traces_preserved; try apply H. i. s. congruence.
+      * ii. clarify. special H0; ss. clarify.
+    + ii. ss. inv STEP0; ss; ModSem.tac. inv FINAL; ss; ModSem.tac.
+    + ii. inv H; ss; ModSem.tac. exploit sd_traces_at; eauto.
+Qed.
+
+Lemma lift_dstar
+      (ms: ModSem.t) st0 tr st1 prog
+      (PUBEQ: ms.(symbolenv).(Senv.public_symbol) = (Sem.sem prog).(symbolenv).(Senv.public_symbol))
+      (DSTAR: DStar ms st0 tr st1):
+    forall tail,
+    <<DSTAR: DStar (Sem.sem prog) (State ((Frame.mk ms st0) :: tail)) tr (State ((Frame.mk ms st1) :: tail))>>.
+Proof.
+  i. ginduction DSTAR; ii; ss.
+  - econs 1; eauto.
+  - clarify. econs 2; eauto.
+    + eapply lift_dstep; eauto.
+    + eapply IHDSTAR; eauto.
+Qed.
+
+Lemma lift_dplus
+      (ms: ModSem.t) st0 tr st1 prog
+      (PUBEQ: ms.(symbolenv).(Senv.public_symbol) = (Sem.sem prog).(symbolenv).(Senv.public_symbol))
+      (DPLUS: DPlus ms st0 tr st1):
+    forall tail,
+    <<DPLUS: DPlus (Sem.sem prog) (State ((Frame.mk ms st0) :: tail)) tr (State ((Frame.mk ms st1) :: tail))>>.
+Proof.
+  i. inv DPLUS; ii; ss. econs; eauto.
+  - eapply lift_dstep; eauto.
+  - eapply lift_dstar; eauto.
+Qed.
+
+Lemma lift_receptive_at
+      (ms: ModSem.t) st0 prog
+      (PUBEQ: ms.(symbolenv).(Senv.public_symbol) = (Sem.sem prog).(symbolenv).(Senv.public_symbol))
+      (RECEP: receptive_at ms st0):
+    forall tail, <<RECEP: receptive_at (Sem.sem prog) (State ((Frame.mk ms st0) :: tail))>>.
+Proof.
+  ii. inv RECEP. ss. econs; eauto; ii.
+  - inv H.
+    + eapply match_traces_nil_l in H0; subst. esplits; eauto. econs 1; eauto.
+    + ss. exploit sr_receptive_at; eauto.
+      { eapply match_traces_preserved; try apply H0. i. s. congruence. }
+      i; des. esplits; eauto. econs; eauto.
+    + eapply match_traces_nil_l in H0; subst. esplits; eauto. econs 4; eauto.
+  - inv H; s; try omega. exploit sr_traces_at; eauto.
+Qed.
+
+Lemma lift_determinate_at
+      (ms: ModSem.t) st0 prog
+      (PUBEQ: ms.(symbolenv).(Senv.public_symbol) = (Sem.sem prog).(symbolenv).(Senv.public_symbol))
+      (DTM: determinate_at ms st0):
+    forall tail,
+    <<DTM: determinate_at (Sem.sem prog) (State ((Frame.mk ms st0) :: tail))>>.
+Proof.
+  ii. inv DTM. ss. econs; eauto; ii.
+  - inv H; inv H0; ModSem.tac.
+    + esplits; et.
+      { eapply match_traces_nil_nil; et. }
+      i. f_equal. eapply ModSem.at_external_dtm; et.
+    + ss. determ_tac sd_determ_at. esplits; et.
+      { eapply match_traces_preserved; try apply H. i. s. congruence. }
+      i. clarify. repeat f_equal. eauto.
+    + ss. esplits; et.
+      { eapply match_traces_nil_nil; et. }
+      i. repeat f_equal. determ_tac ModSem.final_frame_dtm. eapply ModSem.after_external_dtm; et.
+  - ss. inv FINAL. ss. inv STEP; ss; ModSem.tac.
+  - inv H; s; try omega. exploit sd_traces_at; eauto.
+Qed.
+
+(* Lemma callstate_receptive_at *)
+(*       prog *)
+(*       args frs *)
+(*   : *)
+(*     <<RECEP: receptive_at (Sem.sem prog) (Callstate args frs)>> *)
+(* . *)
+(* Proof. *)
+(*   econs; eauto. *)
+(*   - ii. ss. des_ifs. *)
+(*     + inv H. inv H0. esplits; eauto. econs; eauto. *)
+(*     + inv H. inv MSFIND. ss. *)
+(*   - ii. inv H. ss. omega. *)
+(* Qed. *)
+
+(* Lemma callstate_determinate_at *)
+(*       prog *)
+(*       args frs *)
+(*   : *)
+(*     <<RECEP: determinate_at (Sem.sem prog) (Callstate args frs)>> *)
+(* . *)
+(* Proof. *)
+(*   econs; eauto. *)
+(*   - ii. ss. des_ifs. *)
+(*     + inv H. inv H0. esplits; eauto. *)
+(*       * econs; eauto. *)
+(*       * i. repeat f_equal. clear_tac. *)
+(*         exploit find_fptr_owner_determ; eauto. *)
+(*         { ss. rewrite Heq. eapply MSFIND. } *)
+(*         { ss. rewrite Heq. eapply MSFIND0. } *)
+(*         i; clarify. *)
+(*         determ_tac ModSem.initial_frame_dtm. *)
+(*     + exfalso. inv H. inv MSFIND. ss. *)
+(*   - ii. ss. des_ifs. *)
+(*     + inv FINAL. *)
+(*     + inv FINAL. *)
+(*   - ii. inv H. ss. omega. *)
+(* Qed. *)
+
+Section WFMEM.
+
+  Lemma link_load_skenv_wf_mem
+        p sk_link m_init
+        (LINK: link_sk p = Some sk_link)
+        (WF: forall md (IN: In md p), Sk.wf md)
+        (LOADM: Sk.load_mem sk_link = Some m_init):
+    let skenv_link := Sk.load_skenv sk_link in
+    <<WFM: forall md (IN: In md p), SkEnv.wf_mem skenv_link md m_init>>.
+  Proof.
+    ii. eapply SkEnv.load_skenv_wf_mem; et.
+    { eapply link_list_preserves_wf_sk; et. }
+    { unfold link_sk in *. hexploit (link_list_linkorder _ LINK); et. intro T; des.
+      rewrite Forall_forall in T. eapply T; et. rewrite in_map_iff. esplits; et. }
+  Qed.
+
+End WFMEM.
+
+
+Require Import Sem SimModSem.
+Theorem safe_implies_safe_modsem
+        p sk ms lst tail
+        (LINK: link_sk p = Some sk)
+        (SAFE: safe (sem p) (State ({| Frame.ms := ms; Frame.st := lst |} :: tail))):
+    <<SAFE: safe_modsem ms lst>>.
+Proof.
+  ii. ss. exploit SAFE.
+  { instantiate (1:= (State ({| Frame.ms := ms; Frame.st := st1 |} :: tail))). eapply lift_star; eauto. }
+  i; des.
+  - ss. inv H. ss. right. left. eauto.
+  - ss. des_ifs. inv H; ss.
+    + left. eauto.
+    + right. right. eauto.
+    + right. left. eauto.
+Qed.
+
+
+Lemma backward_simulation_refl: forall SEM, backward_simulation SEM SEM.
+Proof.
+  i. eapply (@Backward_simulation _ _ unit bot2). econs; eauto.
+  { apply unit_ord_wf. }
+  ii. ss. exists tt. esplits; eauto.
+  clear st_init_src_ INITSRC INITTGT. rename st_init_tgt into st. revert st.
+  pcofix CIH. i. pfold. econs; eauto.
+  ii. econs; eauto.
+  { ii. esplits; eauto. left. apply plus_one. ss. }
+  { i. r in SAFESRC. specialize (SAFESRC st (star_refl _ _ _ _)). ss. }
+  { ii. esplits; eauto. econs; eauto. }
+Qed.
+
+Lemma sk_nwf_improves (mds_src mds_tgt: program)
+      (NWF: ~ (forall x (IN: In x mds_src), Sk.wf x)):
+      improves (sem mds_src) (sem mds_tgt).
+Proof.
+  eapply bsim_improves. econs. econs; try (i; inv INITSRC; clarify). eapply unit_ord_wf.
+Qed.
