theories/SimMod.v
@@ -1,0 +1,54 @@
+Require Import Parameters.
+Require Import Smallstep.
+Require Import CoqlibC.
+Require Import ModSem.
+Require Import LinkingC.
+
+Require Import Syntax Sem Mod ModSem.
+Require Import Sound.
+Require Import SimSymb SimMem SimModSem.
+
+Set Implicit Arguments.
+
+
+
+
+
+
+
+Module ModPair.
+
+Section MODPAIR.
+Context `{SM: SimMem.class} {SS: SimSymb.class SM} {SU: Sound.class}.
+
+  Record t: Type := mk {
+    src: Mod.t;
+    tgt: Mod.t;
+    ss: SimSymb.t;
+  }.
+
+  Definition to_msp (skenv_link_src skenv_link_tgt: SkEnv.t) (sm: SimMem.t) (mp: t): ModSemPair.t :=
+    ModSemPair.mk (Mod.modsem (mp.(src)) skenv_link_src) (Mod.modsem (mp.(tgt)) skenv_link_tgt) mp.(ss) sm.
+
+  (* TODO: Actually, ModPair can have idx/ord and transfer it to ModSemPair. *)
+  (* Advantage: We can unify ord at Mod state. *)
+  Inductive sim (mp: t): Prop :=
+  | sim_intro
+      (SIMSK: SimSymb.wf mp.(ss))
+      (SKSRC: mp.(ss).(SimSymb.src) = (Mod.sk mp.(src)))
+      (SKTGT: mp.(ss).(SimSymb.tgt) = (Mod.sk mp.(tgt)))
+      (SIMMS: forall skenv_link_src skenv_link_tgt ss_link sm_init_link
+          (INCLSRC: SkEnv.includes skenv_link_src (Mod.sk mp.(src)))
+          (INCLTGT: SkEnv.includes skenv_link_tgt (Mod.sk mp.(tgt)))
+          (WFSRC: SkEnv.wf skenv_link_src)
+          (WFTGT: SkEnv.wf skenv_link_tgt)
+          (SSLE: SimSymb.le mp.(ss) ss_link)
+          (SIMSKENVLINK: SimSymb.sim_skenv sm_init_link ss_link skenv_link_src skenv_link_tgt),
+          <<SIMMSP: ModSemPair.sim (to_msp skenv_link_src skenv_link_tgt sm_init_link mp)>>).
+
+  (* Design: ModPair only has data, properties are stated in sim *)
+
+End MODPAIR.
+End ModPair.
+
+Hint Unfold ModPair.to_msp.
