README.md
@@ -1,0 +1,9 @@
+Based on:
+CompCertR - d7b3362e7f087b4a29345f4d235dd56ca0940d3f
+CompCertM - 1bf2113b2381df604a3abcce7711af1f154d1620
+Coq - 8.10.1 (November 2019)
+
+
+Delta:
+- Genv.symbol_address does not take offset arg
+- Genv.map_defs ignore "block"
